theories/Nogood.v
@@ -6,12 +6,15 @@ Open Scope Z_scope.
 
 Fixpoint satisfies_nogood (x : list Atomic) (sol : Assignment) :=
   match x with
-  | nil => false
+  | nil => Some false
   | a :: xs =>
       let maybe_value := find_value sol (var a) in
       match maybe_value with
-      | Some v => if test_atomic a v then true else satisfies_nogood xs sol
-      | None => false
+      | Some v =>
+          if test_atomic a v
+          then Some true
+          else satisfies_nogood xs sol
+      | None => None
       end
   end.
 
