theories/Variable.v
@@ -3,17 +3,15 @@ Require Import List.
 Require Import String.
 Require Import ZArith.
 
-Definition non_zero_Z := { n : nat | n <> 0 }.
-
 Record IntervalVariable := 
   {
     name : string;
     lower_bound : Z;
-    size: non_zero_Z;
-    upper_bound : Z := lower_bound + Z.of_nat (proj1_sig size)
+    size: nat;
+    upper_bound : Z := lower_bound + Z.of_nat size
   }.
 
-Compute upper_bound {| name := "a"; lower_bound := 1; size := exist _ 5 (Nat.neq_succ_0 4) |}.
+Compute upper_bound {| name := "a"; lower_bound := 1; size := 5 |}.
 
 Open Scope Z_scope.
 
@@ -22,8 +20,93 @@ Inductive Var :=
 
 Definition eqb (lhs : Var) (rhs : Var) :=
   match (lhs, rhs) with
-  | (interval lhs, interval rhs) => String.eqb (name lhs) (name rhs)
+  | (interval lhs, interval rhs) => andb
+      (andb (String.eqb (name lhs) (name rhs)) (Z.eqb (lower_bound lhs) (lower_bound rhs)))
+      (Z.eqb (upper_bound lhs) (upper_bound rhs))
   end.
+
+Theorem eqb_eq : forall (a b : Var), Is_true (eqb a b) <-> a = b.
+Proof.
+  intros a b.
+  unfold eqb.
+  destruct a as [[a]], b as [[b]].
+  split.
+  - intros Heq.
+    unfold upper_bound in Heq.
+    simpl in Heq.
+    fold upper_bound0 in Heq.
+    fold upper_bound1 in Heq.
+    apply Is_true_eq_true, andb_prop in Heq.
+    destruct Heq as [Heq Hub].
+    apply andb_prop in Heq.
+    destruct Heq as [Hname Hlb].
+    apply String.eqb_eq in Hname.
+    apply Z.eqb_eq in Hlb.
+    apply Z.eqb_eq in Hub.
+    f_equal.
+    f_equal.
+    + apply Hname.
+    + apply Hlb.
+    + unfold upper_bound0, upper_bound1 in Hub.
+      rewrite Hlb in Hub.
+      apply Z.add_reg_l, Nat2Z.inj in Hub.
+      apply Hub.
+  - intros Heq.
+    inversion Heq.
+    unfold upper_bound.
+    apply Is_true_eq_left.
+    simpl.
+    apply andb_true_intro.
+    split.
+    apply andb_true_intro.
+    split.
+    + apply String.eqb_eq. reflexivity.
+    + apply Z.eqb_eq. reflexivity.
+    + apply Z.eqb_eq. reflexivity.
+Qed.
+
+Theorem eqb_symm : forall (a b : Var), eqb a b = eqb b a.
+Proof.
+  intros a b.
+  unfold eqb.
+  destruct a as [a],  b as [b].
+  rewrite String.eqb_sym, Z.eqb_sym.
+  rewrite Z.eqb_sym with (x := upper_bound b) (y := upper_bound a).
+  reflexivity.
+Qed.
+
+Theorem eqb_trans : forall (a b c : Var), Is_true (eqb a b) -> Is_true(eqb b c) -> Is_true(eqb a c).
+Proof.
+  unfold eqb.
+  intros a b c Hab Hbc.
+  destruct a as [a], b as [b], c as [c].
+  apply Is_true_eq_true, andb_prop in Hab.
+  destruct Hab as [Hab Hab_ub].
+  apply andb_prop in Hab.
+  destruct Hab as [Hab_name Hab_lb].
+  apply Is_true_eq_true, andb_prop in Hbc.
+  destruct Hbc as [Hbc Hbc_ub].
+  apply andb_prop in Hbc.
+  destruct Hbc as [Hbc_name Hbc_lb].
+  apply Is_true_eq_left, andb_true_intro. split.
+  apply andb_true_intro. split.
+  - apply String.eqb_eq in Hab_name.
+    apply String.eqb_eq in Hbc_name.
+    apply String.eqb_eq.
+    rewrite Hab_name.
+    apply Hbc_name.
+  - apply Z.eqb_eq in Hab_lb.
+    apply Z.eqb_eq in Hbc_lb.
+    apply Z.eqb_eq.
+    rewrite Hab_lb.
+    apply Hbc_lb.
+  - apply Z.eqb_eq in Hab_ub.
+    apply Z.eqb_eq in Hbc_ub.
+    apply Z.eqb_eq.
+    rewrite Hab_ub.
+    apply Hbc_ub.
+Qed.
+
 
 Definition var_lower_bound (x : Var) :=
   match x with
